More Fixpoint fun.

src/Examples/DnsServer/RecursiveDNSSchema.v
@@ -189,7 +189,7 @@ Section FixComp.
   Definition funDef (fSig : funSig) :=
     funType (funDom fSig) (funCod fSig).
 
-  Fixpoint SubsetFun
+  Fixpoint refineFun
            {fDom : list Type}
            {fCod : Type}
            (fSet' fSet : funType fDom fCod)
@@ -203,7 +203,7 @@ Section FixComp.
       fun fSet' fSet => refine fSet' fSet
     | cons T fDom' =>
       fun fSet' fSet => 
-        forall (t : T), SubsetFun (fSet' t) (fSet t)
+        forall (t : T), refineFun (fSet' t) (fSet t)
     end fSet' fSet.
 
   Definition FixedPointP
@@ -212,7 +212,7 @@ Section FixComp.
              (fDef : funType fDom fCod -> funType fDom fCod)
              (fSet : funType fDom fCod)
     : Prop :=
-    SubsetFun (fDef fSet) fSet /\ SubsetFun fSet (fDef fSet).
+    refineFun (fDef fSet) fSet /\ refineFun fSet (fDef fSet).
 
   Definition LeastFixedPointP
              {fDom : list Type}
@@ -222,46 +222,346 @@ Section FixComp.
     : Prop :=
     FixedPointP fDef fSet /\
     forall fSet', FixedPointP fDef fSet'
-                  -> SubsetFun fSet fSet'.
+                  -> refineFun fSet' fSet.
 
-    Fixpoint LeastFixedPoint'
-               (fDom : list Type)
-               {fCod : Type}
-               {struct fDom}
-      : ((funType fDom fCod -> Prop) -> Prop) ->  funType fDom fCod :=
-      match fDom return
-            ((funType fDom fCod -> Prop) -> Prop)
-            -> funType fDom fCod with
-      | nil => fun LFP_P v => (LFP_P (fun cv => computes_to cv v))
-      | cons T fDom' =>
-        fun LFP_P => 
-          fun (t : T) => LeastFixedPoint' fDom' (fun cv => LFP_P (fun cv' => cv (cv' t)))
-      end.
+  Local Transparent computes_to.
+
+(*  Definition LeastFixedPoint {A}
+             (f : Comp A -> Comp A)
+    : Comp A :=
+    fun a => forall (ca : Comp A),
+        In _ (f ca) a.
+
+  Lemma refine_LeastFixedPoint {A}
+    : forall (f : Comp A -> Comp A)
+      (f_monotone : forall rec, refine rec (f rec)),
+      refineEquiv (f (LeastFixedPoint f)) (LeastFixedPoint f).
+  Proof.
+    split; eauto.
+    unfold LeastFixedPoint, refine, computes_to; intros.
+    eapply f_monotone in H; apply H.
+  Defined.
+
+  Fixpoint LeastFixedPointFun'
+           (fDom : list Type)
+           {fCod : Type}
+           {struct fDom}
+    : (funType fDom fCod -> funType fDom fCod) -> funType fDom fCod. 
+    refine match fDom return
+          (funType fDom fCod -> funType fDom fCod)
+          -> funType fDom fCod with
+    | nil => fun fDef => LeastFixedPoint fDef
+    | cons T fDom' =>
+      fun fDef (t : T) => LeastFixedPointFun' fDom' fCod _
+           end.
+    simpl in *.
+    intros.
+    apply LeastFixedPointFun'.
+    intro.
     
-    Definition LeastFixedPoint
-               {fDom : list Type}
-               {fCod : Type}
-               (fDef : funType fDom fCod -> funType fDom fCod)
-      : funType fDom fCod :=
-      LeastFixedPoint' fDom (fun z => exists s, LeastFixedPointP fDef s /\ z s).
+    apply fDef.
+    intros.
+    apply X.
+    apply t.
+  Defined. 
 
-    Definition FibannacciSpec 
-               (rec : funType ((nat : Type) :: @nil Type)%list nat)
-      : funType ((nat : Type) :: @nil Type)%list nat :=
-      fun (n : nat) =>
-        match n with
-        | 0 => ret 0
-        | 1 => ret 1
-        | S (S n') => n1 <- rec n';
-                      n2 <- rec (S n');
-                      ret (n1 + n2)
-        end.
 
-                     
-      unfold funType. 
-        funType (nat :: nat :: nil) nat.
+   Definition LeastFixedPointFun
+             {fDom : list Type}
+             {fCod : Type}
+             (fDef : funType fDom fCod -> funType fDom fCod)
+    : funType fDom fCod :=
+    LeastFixedPointFun' fDom fDef.
+
+  Lemma refine_LeastFixedPointFun
+        {fDom : list Type}
+        {fCod : Type}
+        (fDef fDef' : funType fDom fCod -> funType fDom fCod)
+      : respectful (@refineFun fDom fCod)
+                   (@refineFun fDom fCod)
+                   fDef fDef'
+        -> refineFun (LeastFixedPointFun fDef)
+                     (LeastFixedPointFun fDef').
+  Proof.
+    induction fDom; simpl; intros.
+    - unfold LeastFixedPointFun; simpl in *.
+      unfold refine; intros v Comp_v; intuition.
+      unfold computes_to, LeastFixedPoint,
+      FixedPointP, respectful in *; simpl in *.
+      intros.
+      eapply H; eauto.
+      2: eapply (Comp_v ca).
+      reflexivity.
+    - simpl in *.
+      eapply IHfDom; eauto.
+      unfold respectful in *; intros.
+      eapply H.
+      intro.
+      apply H0.
+  Qed.
+
+
+*)
     
-Section DecomposeEnumField.
+  Fixpoint LeastFixedPoint'
+           (fDom : list Type)
+           {fCod : Type}
+           {struct fDom}
+    : ((funType fDom fCod -> Prop) -> Prop) ->  funType fDom fCod :=
+    match fDom return
+          ((funType fDom fCod -> Prop) -> Prop)
+          -> funType fDom fCod with
+    | nil => fun LFP_P v => (LFP_P (fun cv => computes_to cv v))
+    | cons T fDom' =>
+      fun LFP_P => 
+        fun (t : T) => LeastFixedPoint' fDom' (fun cv => LFP_P (fun cv' => cv (cv' t)))
+    end.
+
+  Definition LeastFixedPoint''
+             {fDom : list Type}
+             {fCod : Type}
+             (fDef : funType fDom fCod -> funType fDom fCod)
+    : funType fDom fCod :=
+    LeastFixedPoint' fDom (fun z => exists s, LeastFixedPointP fDef s /\ z s).
+
+  Definition FibonacciSpec 
+    : funType ((nat : Type) :: @nil Type)%list nat :=
+    LeastFixedPoint'' (fDom := (nat : Type) :: @nil Type)%list
+      (fun rec (n : nat) =>
+         match n with
+         | 0 => ret 0
+         | 1 => ret 1
+         | S (S n') =>
+           n1 <- rec n';
+           n2 <- rec (S n');
+           ret (n1 + n2)
+         end).
+
+  Fixpoint FibonacciImpl
+           (n : nat)
+    : Comp nat :=
+    match n with
+    | 0 => ret 0
+    | (S p) => 
+      match p with
+      | 0 => ret 1
+      | (S m) => n1 <- FibonacciImpl p;
+                 n2 <- FibonacciImpl m;
+                 ret (n1 + n2)
+      end
+    end.  
+
+  Lemma foo
+    : refineFun FibonacciSpec FibonacciImpl.
+  Proof.
+    unfold refineFun; unfold refine; intros.
+    unfold FibonacciSpec, LeastFixedPoint''; simpl.
+    unfold LeastFixedPointP, FixedPointP, computes_to; simpl.
+    exists FibonacciImpl; split; eauto.
+    clear H.
+    intuition.
+    admit.
+    admit.
+    admit.
+  Admitted.
+  (*rewrite H1.
+    induction t0.
+    - reflexivity.
+    - simpl.
+      assert (refine (fSet' t0) (FibonacciImpl t0)).
+      intros; rewrite H1.
+      apply IHt0.
+      revert H.
+      destruct t0; intros.
+      * reflexivity.
+      * simpl in *.
+        setoid_rewrite H.
+        intros v' Comp_v'.
+        computes_to_inv; subst.
+        rewrite H1.
+        eapply BindComputes with (a := v1); 
+        repeat computes_to_econstructor.
+        2: apply Comp_v'.
+        2: rewrite plus_comm; repeat computes_to_econstructor.
+        
+        
+        eapply H1 in IHt0.
+      assert (refine
+                (match t0 with
+                 | 0 => ret 1
+                 | S m => n1 <- match t0 with
+                                | 0 => ret 0
+                                | 1 => ret 1
+                                | S (S n') => n1 <- fSet' n';
+                                              n2 <- fSet' (S n');
+                                              ret (n1 + n2)
+                                end;
+                          n2 <- FibonacciImpl m;
+                          ret (n1 + n2)
+                 end)
+                match t0 with
+                | 0 => ret 1
+                | S m => n1 <- FibonacciImpl t0;
+                         n2 <- FibonacciImpl m;
+                         ret (n1 + n2)
+     end).
+      destruct t0.
+      reflexivity.
+      rewrite IHt0.
+      reflexivity.
+      etransitivity; try eauto.
+      clear H.
+      
+      apply 
+      rewrite <- IHt0.
+      induction t0.
+    reflexivity.
+    rewrite H1.
+    setoid_rewrite H1.
+    rewrite <- IHt0.
+    destruct t0.
+    Focus 2.
+    
+    unfold FibonacciImpl.
+    unfold 
+    - induction t0; simpl in *.
+      + simpl; reflexivity.
+      + induction t0.
+        reflexivity.
+        rewrite <- IHt0.
+
+        intros v Comp_v; computes_to_inv.
+        subst.
+        apply IHt in Comp_v.
+        computes_to_econstructor; eauto.
+        destruct t.
+        computes_to_econstructor; eauto.
+        rewrite plus_comm; computes_to_econstructor.
+        simpl in *.
+        computes_to_inv; subst.
+        repeat computes_to_econstructor.
+        apply Comp_v'0.
+        apply Comp_v.
+        rewrite plus_assoc.
+        rewrite plus_comm.
+        rewrite (plus_comm v1 v2).
+        rewrite plus_assoc.
+        computes_to_econstructor; eauto.
+      + induction t.
+        * reflexivity.
+        * simpl.
+          destruct t; eauto.
+          reflexivity.
+          rewrite IHt.
+          induction t.
+          intros v Comp_v.
+          simpl in *; computes_to_inv; subst.
+          repeat computes_to_econstructor; eauto.
+          simpl in *.
+          simpl in 
+          apply IHt in Comp_v.
+          computes_to_econstructor; eauto.
+          destruct t.
+          computes_to_econstructor; eauto.
+          rewrite plus_comm; computes_to_econstructor.
+          simpl in *.
+          computes_to_inv; subst.
+          repeat computes_to_econstructor.
+          apply Comp_v'0.
+          apply Comp_v.
+          rewrite plus_assoc.
+          rewrite plus_comm.
+          rewrite (plus_comm v1 v2).
+          rewrite plus_assoc.
+          computes_to_econstructor; eauto.
+        
+        reflexivity.
+        simpl.
+        
+        setoid_rewrite <- IHt.
+      intros.
+    
+        simpl.
+    
+    - unfold FibonacciSpec, LeastFixedPoint''; simpl.
+        unfold LeastFixedPointP, FixedPointP; simpl.
+      unfold refine; intros.
+      computes_to_inv; subst.
+      unfold computes_to; intuition.
+      eexists.
+    - unfold FibonacciSpec, LeastFixedPointFun in *; simpl in *.
+      destruct t.
+      + unfold refine, LeastFixedPoint; simpl; intros.
+        computes_to_inv; subst.
+        unfold computes_to; intuition.
+      + simpl in *.    
+        rewrite <- IHt.
+        clear.
+        destruct t; simpl.
+  
+  Lemma refine_LeastFixedPoint''
+        {fDom : list Type}
+        {fCod : Type}
+        (fDef fDef' : funType fDom fCod -> funType fDom fCod)
+        (f_monotone : forall rec rec',
+            refineFun rec rec' 
+            -> refineFun (fDef rec) (fDef rec'))
+      : respectful (@refineFun fDom fCod)
+                   (@refineFun fDom fCod)
+                   fDef fDef'
+        -> refineFun (LeastFixedPoint'' fDef)
+                     (LeastFixedPoint'' fDef').
+  Proof.
+    induction fDom; simpl; intros.
+    - unfold LeastFixedPoint''; simpl in *.
+      unfold refine; intros v Comp_v; intuition.
+      unfold computes_to, FixedPointP, respectful in *; simpl in *.
+      destruct Comp_v as [Fix' [LFP_Fix' computes_to_v] ].
+      unfold LeastFixedPointP, FixedPointP in LFP_Fix'; simpl in *;
+        intuition.
+      exists Fix'; split; eauto.
+      unfold LeastFixedPointP, FixedPointP; repeat split.
+      simpl.
+      etransitivity; eauto.
+      Focus 3.
+      simpl.
+      apply H1.
+      
+      
+      
+      simpl in *.
+      unfold FixedPoint
+
+      exists (LeastFixedPoint fDef).
+      unfold LeastFixedPointP; repeat split.
+      + apply refine_LeastFixedPoint; admit.
+      + apply refine_LeastFixedPoint; admit.
+      + unfold FixedPointP; intros; simpl in *.
+        intros v' Comp_v'.
+        unfold LeastFixedPoint in Comp_v'.
+        apply H0; apply Comp_v'.
+      + unfold LeastFixedPoint; intros.
+        destruct Comp_v; intuition.
+        rewrite H; try reflexivity.
+        unfold LeastFixedPointP in H1; simpl in *.
+        intuition.
+        unfold FixedPointP in H0.
+        admit.
+    - simpl in *.
+      pose (
+      unfold respectful in H.
+      rewrite IHfDom.
+      unfold LeastFixedPoint''; simpl.
+
+      eapply IHfDom; eauto.
+      unfold respectful in *; intros.
+      eapply H.
+      intro.
+      apply H0.
+  Qed.  
+   *)
+
+  Section DecomposeEnumField.
 
   Definition IsComputedField
              {heading}
